More tactics

theories/Logic/Ctl.v
@@ -28,898 +28,921 @@ Section Ctl.
   Context {E C: Type -> Type} {X S: Type}
           {h: Handler E S} {HasStuck: B0 -< C}.
   Notation SP := (ctree E C X -> S -> Prop).
-  
-  (* Lift label predicates to SP *)
-  Definition nowS(p: S -> Prop): SP :=
-    fun _ s => p s.
 
-  (* Predicate on return value *)
-  Definition nowR(p: X -> S -> Prop): SP :=
-    fun t s => exists x, t ≅ Ret x /\ p x s.
-
-  (* Propositional *)
-  Definition cimpl: SP -> SP -> SP :=
-    fun a b t l => a t l -> b t l.
-
-  Definition cand: SP -> SP -> SP :=
-    fun a b t l => a t l /\ b t l.
-
-  Definition cor: SP -> SP -> SP :=
-    fun a b t l => a t l \/ b t l.
-
-  Definition cnot: SP -> SP :=
-    fun a t l => not (a t l).
-  
-  (*| Temporal, inductives |*)
-  (* Forall Next *)
-  Definition ax : SP -> SP :=
-    fun p t s => forall t' s', ktrans (t,s) (t',s') -> p t' s'.
-  
-  (* Forall Next *)
-  Definition ex : SP -> SP :=
-    fun p t s => exists t' s', ktrans (t,s) (t',s') /\ p t' s'.
+  Variant CtlQuantifier: Set := Ex | Fa.
 
   (* Forall strong until *)
-  Inductive au: SP -> SP -> SP :=
+  Inductive cau: SP -> SP -> SP :=
   | MatchA: forall t s (p q: SP),       
       q t s ->  (* Matches [q] now; done *)
-      au p q t s
+      cau p q t s
   | StepA:  forall t s (p q: SP),       
       p t s ->    (* Matches [p] now; steps to (t', s') *)
-      (forall t' s', ktrans (t,s) (t',s') -> au p q t' s') ->
-      au p q t s.
-      
+      (forall t' s', ktrans (t,s) (t',s') -> cau p q t' s') ->
+      cau p q t s.
+                          
   (* Exists strong until *)
-  Inductive eu: SP -> SP -> SP :=
+  Inductive ceu: SP -> SP -> SP :=
   | MatchE: forall t s (p q: SP),
       q t s ->       (* Matches [q] now; done *)
-      eu p q t s
+      ceu p q t s
   | StepE: forall t s (p q: SP),
       p t s ->    (* Matches [p] now; steps to (t', s') *)
-      (exists t' s', ktrans (t,s) (t',s') /\ eu p q t' s') ->
-      eu p q t s.
+      (exists t' s', ktrans (t,s) (t',s') /\ ceu p q t' s') ->
+      ceu p q t s.
+
+  (* Forall release *)
+  Variant carF R: SP -> SP -> SP :=
+  | RMatchA: forall t s (p q: SP),       
+      q t s ->  (* Matches [q] now; done *)
+      p t s ->  (* Matches [p] as well *)
+      carF R p q t s
+  | RStepA:  forall t s (p q: SP),       
+      q t s ->    (* Matches [p] now; steps to (t', s') *)
+      (forall t' s', ktrans (t,s) (t',s') -> R t' s') ->
+      carF R p q t s.
+                          
+  (* Exists release *)
+  Variant cerF R : SP -> SP -> SP :=
+  | RMatchE: forall t s (p q: SP),
+      q t s ->       (* Matches [q] now; done *)
+      p t s ->       (* Matches [p] as well *)
+      cerF R p q t s
+  | RStepE: forall t s (p q: SP),
+      q t s ->    (* Matches [p] now; steps to (t', s') *)
+      (exists t' s', ktrans (t,s) (t',s') /\ R t' s') ->
+      cerF R p q t s.
+
+  Hint Constructors cau ceu carF cerF: core.
   
-  (*| Temporal, Coinductives |*)  
-  (* Forall global *)
-  Definition agF (p: SP)(R: SP): SP :=
-    fun t s => p t s /\ (forall t' s', ktrans (t,s) (t',s') -> R t' s').
+  (*| Global (coinductives) |*)
+  Program Definition car p q: mon SP :=
+    {| body := fun R t s => carF R p q t s |}.
+  Next Obligation. destruct H0; auto. Qed.
+  
+  Program Definition cer p q: mon SP :=
+    {| body := fun R t s => cerF R p q t s |}.
+  Next Obligation. destruct H0; [eauto | destruct H1 as (t' & s' & TR & ?)]; apply RStepE; eauto. Qed.
+  
+  Inductive CtlFormula: Type :=
+  | CNowS (p : S -> Prop): CtlFormula
+  | CNowR (p : X -> S -> Prop): CtlFormula
+  | CAnd    : CtlFormula -> CtlFormula -> CtlFormula
+  | COr     : CtlFormula -> CtlFormula -> CtlFormula
+  | CImpl   : CtlFormula -> CtlFormula -> CtlFormula
+  | CAX     : CtlFormula -> CtlFormula
+  | CEX     : CtlFormula -> CtlFormula
+  | CAU     : CtlFormula -> CtlFormula -> CtlFormula
+  | CEU     : CtlFormula -> CtlFormula -> CtlFormula
+  | CAR     : CtlFormula -> CtlFormula -> CtlFormula
+  | CER     : CtlFormula -> CtlFormula -> CtlFormula.
 
-  (* Exists global *)
-  Definition egF (p: SP) (R: SP): SP :=
-    fun t s => p t s /\ (exists t' s', ktrans (t,s) (t',s') /\ R t' s').
+  (* Entailment inductively on formulas *)
+  Fixpoint entailsF (φ: CtlFormula): ctree E C X -> S -> Prop :=
+    match φ with
+    | CNowS p   => fun _ s => p s
+    | CNowR q   => fun t s => exists (x: X), t ≅ Ret x /\ q x s
+    | CAnd  φ ψ => fun t s => (entailsF φ t s) /\ (entailsF ψ t s)
+    | COr   φ ψ => fun t s => (entailsF φ t s) \/ (entailsF ψ t s)
+    | CImpl φ ψ => fun t s => (entailsF φ t s) -> (entailsF ψ t s)
+    | CAX   φ   => fun t s =>  forall t' s', ktrans (t,s) (t',s') -> entailsF φ t' s'
+    | CEX   φ   => fun t s =>  exists t' s', ktrans (t,s) (t',s') /\ entailsF φ t' s'
+    | CAU   φ ψ => cau (entailsF φ) (entailsF ψ)
+    | CEU   φ ψ => ceu (entailsF φ) (entailsF ψ)
+    | CAR   φ ψ  => gfp (car (entailsF φ) (entailsF ψ))
+    | CER   φ ψ  => gfp (cer (entailsF φ) (entailsF ψ))
+    end.
 
-  Definition entails(p: SP) (t: ctree E C X)(s: S): Prop := p t s.
- 
-  Arguments agF /.
-  Arguments egF /.
-    
-  Program Definition ag_ p: mon SP := {| body := agF p |}.
-  Program Definition eg_ p: mon SP := {| body := egF p |}.  
-  Next Obligation. esplit; eauto. Qed.
-
-  Definition ag p := (gfp (@ag_ p)).
-  Definition eg p := (gfp (@eg_ p)).
 End Ctl.
 
 Module CtlNotations.
 
   Declare Custom Entry ctl.
   Declare Scope ctl_scope.
-
+  Delimit Scope ctl_scope with ctl.
+  
   Section SC.
     Context {E C: Type -> Type} {X S: Type}.
     Notation SP := (ctree E C X -> S -> Prop).
-    Definition ctl_of_Prop (P : Prop) : SP := nowS (fun (_: S) => P).
-    Definition ctl_of_State (s: S): SP := nowS (fun (x: S) => x = s).
-    Coercion ctl_of_Prop : Sortclass >-> Funclass. 
-    Coercion ctl_of_State : S >-> Funclass.
+    Definition ctl_of_Prop (P : Prop) : @CtlFormula X S := CNowS (fun (_: S) => P).
+    Coercion ctl_of_Prop : Sortclass >-> CtlFormula. 
   End SC.
   
   Notation "<( e )>" := e (at level 0, e custom ctl at level 95) : ctl_scope.
   Notation "( x )" := x (in custom ctl, x at level 99) : ctl_scope.
   Notation "{ x }" := x (in custom ctl at level 0, x constr): ctl_scope.
   Notation "x" := x (in custom ctl at level 0, x constr at level 0) : ctl_scope.
-  Notation "t , s |= p " := (entails p t s) (in custom ctl at level 80,
-                                                p custom ctl,
-                                                right associativity): ctl_scope.
+  Notation "t , s |= φ " := (entailsF φ t s) (in custom ctl at level 80,
+                                                 φ custom ctl,
+                                                 right associativity): ctl_scope.
+
+  Notation "|- φ " := (entailsF φ) (in custom ctl at level 80,
+                                       φ custom ctl, only parsing): ctl_scope.
+
   (* Temporal *)
-  Notation "'now' p" := (nowS p) (in custom ctl at level 79): ctl_scope.
-  Notation "'ret' p" := (nowR p) (in custom ctl at level 79): ctl_scope.
-  Notation "'EX' p" := (ex p) (in custom ctl at level 75): ctl_scope.
-  Notation "'AX' p" := (ax p) (in custom ctl at level 75): ctl_scope.
-  Notation "p 'EU' q" := (eu p q) (in custom ctl at level 75): ctl_scope.
-  Notation "p 'AU' q" := (au p q) (in custom ctl at level 75): ctl_scope.
-  Notation "'EF' p" := (eu True p) (in custom ctl at level 75): ctl_scope.
-  Notation "'AF' p" := (au True p) (in custom ctl at level 75): ctl_scope.
-  Notation "'EG' p" := (eg p) (in custom ctl at level 75): ctl_scope.
-  Notation "'AG' p" := (ag p) (in custom ctl at level 75): ctl_scope.
+  Notation "'now' p" := (CNowS p) (in custom ctl at level 79): ctl_scope.
+  Notation "'ret' p" := (CNowR p) (in custom ctl at level 79): ctl_scope.
+  Notation "'EX' p" := (CEX p) (in custom ctl at level 75): ctl_scope.
+  Notation "'AX' p" := (CAX p) (in custom ctl at level 75): ctl_scope.
+  Notation "'EF' p" := (CEU True p) (in custom ctl at level 74): ctl_scope.
+  Notation "'AF' p" := (CAU True p) (in custom ctl at level 74): ctl_scope.
+  Notation "'EG' p" := (CER False p) (in custom ctl at level 74): ctl_scope.
+  Notation "'AG' p" := (CAR False p) (in custom ctl at level 74): ctl_scope.
+  Notation "p 'EU' q" := (CEU p q) (in custom ctl at level 75): ctl_scope.
+  Notation "p 'AU' q" := (CAU p q) (in custom ctl at level 75): ctl_scope.
+  Notation "p 'ER' q" := (CER p q) (in custom ctl at level 75): ctl_scope.
+  Notation "p 'AR' q" := (CAR p q) (in custom ctl at level 75): ctl_scope.
 
   (* Propositional *)
-  Notation "p '/\' q" := (cand p q) (in custom ctl at level 77, left associativity): ctl_scope.
-  Notation "p '\/' q" := (cor p q) (in custom ctl at level 77, left associativity): ctl_scope.
-  Notation "p '->' q" := (cimpl p q) (in custom ctl at level 78, right associativity): ctl_scope.
-  Notation "p '<->' q" := (cand (cimpl p q) (cimpl q p))
-                            (in custom ctl at level 77): ctl_scope.
+  Notation "p '/\' q" := (CAnd p q) (in custom ctl at level 77, left associativity): ctl_scope.
+  Notation "p '\/' q" := (COr p q) (in custom ctl at level 77, left associativity): ctl_scope.
+  Notation "p '->' q" := (CImpl p q) (in custom ctl at level 78, right associativity): ctl_scope.
+  Notation "p '<->' q" := (CAnd (CImpl p q) (CImpl q p)) (in custom ctl at level 77): ctl_scope.
 
   (* Companion notations *)
-  Notation agt p := (t (ag_ p)).
-  Notation agbt p := (bt (ag_ p)).
-  Notation egt p := (t (eg_ p)).
-  Notation egbt p := (bt (eg_ p)).
-  Notation agT p := (T (ag_ p)).
-  Notation egT p := (T (eg_ p)).
-  Notation agbT p := (bT (ag_ p)).
-  Notation egbT p := (bT (eg_ p)).
+  Notation cart p q := (t (car p q)).
+  Notation carbt p q := (bt (car p q)).
+  Notation cert p q := (t (cer p q)).
+  Notation cerbt p q := (bt (cer p q)).
+  Notation carT p q := (T (car p q)).
+  Notation cerT p q := (T (cer p q)).
+  Notation carbT p q := (bT (car p q)).
+  Notation cerbT p q := (bT (cer p q)).
 
   (* TODO: Think proof lemmas so these don't escape to the user? *)
-  Notation "[ 'AG' ] p" := (ag_ p _) (in custom ctl at level 75, p custom ctl): ctl_scope.
-  Notation "[ 'EG' ] p" := (eg_ p _) (in custom ctl at level 75, p custom ctl): ctl_scope.
+  Notation "p [ 'AR' ] q" := (car p q _) (in custom ctl at level 75,
+                                             p custom ctl, q custom ctl): ctl_scope.
+  Notation "p [ 'ER' ] q" := (cer p q _) (in custom ctl at level 75,
+                                             p custom ctl, q custom ctl): ctl_scope.
   
-  Notation "[[ 'AG' ]] p" := (agF p _) (in custom ctl at level 75, p custom ctl): ctl_scope.
-  Notation "[[ 'EG' ]] p" := (egF p _) (in custom ctl at level 75, p custom ctl): ctl_scope.
+  Notation "p [[ 'AR' ]] q" := (car.(body) p q _) (in custom ctl at level 75,
+                                                      p custom ctl, q custom ctl): ctl_scope.
+  Notation "p [[ 'ER' ]] q" := (cer.(body) p q _) (in custom ctl at level 75,
+                                                      p custom ctl, q custom ctl): ctl_scope.
   
-  Notation "{ 'AG' } p" := (agt p _) (in custom ctl at level 75, p custom ctl): ctl_scope.
-  Notation "{ 'EG' } p" := (egt p _) (in custom ctl at level 75, p custom ctl): ctl_scope.
+  Notation "p { 'AR' } q" := (cart p q _) (in custom ctl at level 75,
+                                              p custom ctl, q custom ctl): ctl_scope.
+  Notation "p { 'ER' } q" := (cert p q _) (in custom ctl at level 75,
+                                              p custom ctl, q custom ctl): ctl_scope.
   
-  Notation "{{ 'AG' }} p" := (agbt p _) (in custom ctl at level 75, p custom ctl): ctl_scope.
-  Notation "{{ 'EG' }} p" := (egbt p _) (in custom ctl at level 75, p custom ctl): ctl_scope.
-  
-End CtlNotations.
-  
-Import CtlNotations.
+  Notation "p {{ 'AR' }} q" := (carbt p q _) (in custom ctl at level 75,
+                                                 p custom ctl, q custom ctl): ctl_scope.
+  Notation "p {{ 'ER' }} q" := (cerbt p q _) (in custom ctl at level 75,
+                                                 p custom ctl, q custom ctl): ctl_scope.
 
-#[global] Hint Constructors eu au: core.
-#[global] Hint Unfold cand cor cimpl ax ex nowS nowR: core.
-Arguments cand /.
-Arguments cor /.
-Arguments cimpl /.
-Arguments ax /.
-Arguments ex /.
-Arguments agF /.
-Arguments egF /.
-Arguments nowS /.
-Arguments nowR /.
-Arguments entails: simpl never.
+  #[global] Hint Constructors ceu cau: core.
+  Arguments entailsF: simpl never.
+End CtlNotations.
+
+
+
+(* Properness lemmas/ Up-to proofs *)
+Tactic Notation "step_entails" :=
+  match goal with
+  | |- context[@entailsF ?E ?C ?X ?Σ ?h ?HasStuck] =>
+      progress (unfold entailsF; cbn; fold (@entailsF E C X Σ h HasStuck))
+  end.
+Tactic Notation "step_entails" "in" ident(H) :=
+  match type of H with
+  | context[@entailsF ?E ?C ?X ?Σ ?h ?HasStuck] =>
+      progress (unfold entailsF in H; cbn in H; fold (@entailsF E C X Σ h HasStuck) in H)
+  end.
+
+(* these acrobatics are because Ltac does not make it easy to match a [fix] *)
+Tactic Notation "fold_entails" :=
+  match goal with
+  | |- ?F ?φ ?t ?s => 
+      match type of F with
+      | (@CtlFormula ?X ?Σ) -> (ctree ?E ?C ?X) -> ?Σ -> Prop =>
+          is_fix F; progress fold (@entailsF E C X Σ _ _ φ t s)
+      end
+  end.
+
+Tactic Notation "fold_entails" "in" ident(H) :=
+  match type of H with
+  | ?F ?φ ?t ?s => 
+      match type of F with
+      | (@CtlFormula ?X ?Σ) -> (ctree ?E ?C ?X) -> ?Σ -> Prop =>
+          is_fix F; progress fold (@entailsF E C X Σ _ _ φ t s) in H
+      end
+  end.
 
 (*| Equations of CTL |*)
 Section Equivalences.
+  Import CtlNotations.
   Local Open Scope ctl_scope.
-  Context {E C: Type -> Type} {X S: Type} {HasStuck: B0 -< C} {h: Handler E S}.
-
-  (* Kripke state predicates *)
-  Notation SP := (ctree E C X -> S -> Prop).
+  Context {E C: Type -> Type} {X Σ: Type} {HasStuck: B0 -< C} {h: Handler E Σ}.
 
   (* SP is proper setoid *)
-  Program Instance SpSetoid : Setoid SP :=
-    {| equiv := fun P Q => forall (t: ctree E C X) (s:S), P t s <-> Q t s |}.
+  Program Instance SpSetoid: Setoid CtlFormula :=
+    {| equiv := fun P Q => forall (t: ctree E C X) (s:Σ),
+                    <( t, s |= P )> <-> <( t, s |= Q )> |}.
   Next Obligation.
     split.
     - intros P x; reflexivity.
-    - intros P Q H x s; symmetry; auto.
-    - intros P Q R H0 H1 x s; transitivity (Q x s); auto.
+    - intros P Q H' x s; symmetry; auto.
+    - intros P Q R H0' H1' x s; transitivity <(x, s |= Q)>%ctl; auto.
   Qed.
 
+  #[global] Instance proper_equiv_equiv:
+    Proper (SpSetoid.(equiv) ==> SpSetoid.(equiv) ==> iff) SpSetoid.(equiv).
+  Proof.
+    do 3 red; split; intros; do 2 red in H, H0, H1; do 2 red; split; intros.
+    - now rewrite <- H0, <- H1, H. 
+    - now rewrite <- H, H1, H0.
+    - now rewrite H0, <- H1, <- H.
+    - now rewrite H, H1, <- H0.
+  Qed.
+  
   (*| Top is True |*)
-  Lemma ctl_top: forall (t: ctree E C X) (s: S),
+  Lemma ctl_top: forall (t: ctree E C X) (s: Σ),
     <( t, s |= True )>.
   Proof. reflexivity. Qed.    
 
   (*| Bot is False |*)
-  Lemma ctl_bot: forall (t: ctree E C X) (s: S),
+  Lemma ctl_bot: forall (t: ctree E C X) (s: Σ),
     ~ <(t, s |= False)>.
-  Proof.
+   Proof.
     intros * CONTRA; apply CONTRA.
   Qed.
 
   (*| Ex-falso |*)
-  Lemma ctl_ex_falso: forall (t: ctree E C X) (s: S) p,
+  Lemma ctl_ex_falso: forall (t: ctree E C X) (s: Σ) p,
       <( t,s |= False -> p )>.
   Proof.
-    intros * CONTRA; contradiction.
+    intros; unfold entailsF; intro CONTRA; contradiction.
   Qed.
 
-  Lemma ctl_af_ax: forall (p: SP),
-      <( AF p )> == <( p \/ AX (AF p) )>.
-  Proof.
-    split; intros; inv H.
-    - now left.
-    - now right. 
-    - now left. 
-    - now right.
-  Qed.
-
-  Lemma ctl_ef_ex: forall (p: SP),
-      <( EF p )> == <( p \/ EX (EF p) )>.
-  Proof.
-    split; intros; inv H.
-    - now left.
-    - now right. 
-    - now left. 
-    - now right.
-  Qed.
-
-  Lemma ctl_ag_ax: forall (p: SP),
-      <( AG p )> == <( p /\ AX (AG p) )>.
-  Proof. 
-    split; intros.
-    - split; step in H.
-      + now destruct H.
-      + destruct H.
-        unfold ax; auto.
-    - destruct H.
-      red in H0.
-      step.
-      split; eauto; simpl.
-  Qed.
-
-  Lemma ctl_eg_ex: forall (p: SP),
-      <( EG p )> == <( p /\ EX (EG p) )>.
-  Proof. 
-    split; intros.
-    - split; step in H.
-      + now destruct H.
-      + destruct H as (? & t' & l' & ?).
-        unfold ex; eauto.
-    - destruct H as (? & t' & l' & ?).
-      step.
-      split; eauto.
-  Qed.
-
-  Lemma ctl_au_ax: forall (p q: SP),
+  Lemma ctl_au_ax: forall p q,
       <( p AU q )> == <( q \/ (p /\ AX (p AU q)) )>.
   Proof.
     split; intros.
-    - inv H.
-      + now left.
-      + now right.
-    - inv H.
-      + now apply MatchA.
-      + destruct H0; auto.
+    - inv H; [now left | now right].
+    - destruct H; [now apply MatchA | now apply StepA].
   Qed.
 
-  Lemma ctl_eu_ex: forall (p q: SP),
+  Lemma ctl_eu_ex: forall p q,
       <( p EU q )> == <( q \/ (p /\ EX (p EU q)) )>.
   Proof.
     split; cbn; intros.
-    - inv H.
-      + now left.
-      + now right.
-    - inv H.
-      + now apply MatchE.
-      + destruct H0; auto.
+    - inv H; [now left | now right].
+    - inv H; [now apply MatchE | now apply StepE].
+  Qed.
+  
+  Lemma ctl_af_ax: forall p,
+      <( AF p )> == <( p \/ AX (AF p) )>.
+  Proof.
+    split; intros; inv H.
+    1,3 : now left.
+    all: now right. 
   Qed.
 
+  Lemma ctl_ef_ex: forall p,
+      <( EF p )> == <( p \/ EX (EF p) )>.
+  Proof.
+    split; intros; inv H.
+    1,3: now left.
+    all: now right.
+  Qed.
+
+   Lemma ctl_ar_ax: forall p q,
+      <( p AR q )> == <( q /\ (p \/ AX (p AR q)) )>.
+   Proof. 
+     split; intros.
+     - split; step in H; inv H; auto.
+     - step_entails.
+       destruct H  as (? & [? | ?]).
+       + step; now apply RMatchA.
+       + step; apply RStepA; auto.
+  Qed.
+
+   Lemma ctl_er_ex: forall p q,
+      <( p ER q )> == <( q /\ (p \/ EX (p ER q)) )>.
+   Proof. 
+     split; intros.
+     - split; step in H; inv H; auto.
+     - step_entails.
+       destruct H  as (? & [? | ?]).
+       + step; now apply RMatchE.
+       + step; apply RStepE; auto.
+  Qed.
+
+   Lemma ctl_ag_ax: forall p,
+       <( AG p )> == <( p /\ AX (AG p) )>.
+   Proof. 
+     split; intros.
+     - split; step in H; now inv H.
+     - destruct H; step; now apply RStepA.
+   Qed.
+
+  Lemma ctl_eg_ex: forall p,
+      <( EG p )> == <( p /\ EX (EG p) )>.
+  Proof. 
+    split; intros.
+    - split; step in H; now inv H.
+    - destruct H as (? & ? & ? & ? & ?); step; apply RStepE; eauto.
+  Qed.
+  
+  (** Inductive lemmas for AU, EU *)
+  Lemma AU_ind' :
+    forall [φ ψ: CtlFormula] (P : ctree E C X -> Σ -> Prop),
+      (forall t s, <(t, s |= ψ)> -> P t s) -> (* base *)
+      (forall (t: ctree E C X) (s : Σ),
+         <(t, s |= φ )> ->          (* φ now*)
+         (forall t' s', ktrans (t,s) (t',s') -> <(t',s' |= φ AU ψ)>) ->
+         (forall t' s', ktrans (t,s) (t',s') -> P t' s') ->
+         P t s) ->
+      forall t s, <( t, s |= φ AU ψ )> -> P t s.
+  Proof.
+    intros φ ψ P Hbase Hstep.
+    refine (fix F (t : ctree E C X)(s: Σ) (H : <( t, s |= φ AU ψ)>) : P t s := _).
+    remember (entailsF φ) as p.
+    remember (entailsF ψ) as q.
+    step_entails in H.
+    dependent destruction H; subst.
+    - now apply Hbase.
+    - apply Hstep; auto.
+      intros.
+      specialize (H0 _ _ H1).
+      apply F.
+      now step_entails.
+  Qed.  
+
+  Lemma AF_ind' :
+    forall [φ: CtlFormula] (P : ctree E C X -> Σ -> Prop),
+      (forall t s, <(t, s |= φ)> -> P t s) -> (* base *)
+      (forall (t: ctree E C X) (s : Σ),
+          (forall t' s', ktrans (t,s) (t',s') -> <(t',s' |= AF φ)>) ->
+          (forall t' s', ktrans (t,s) (t',s') -> P t' s') ->
+          P t s) ->
+      forall t s, <( t, s |= AF φ )> -> P t s.
+  Proof.
+    intros φ ψ P Hbase Hstep.
+    eapply AU_ind'; eauto.
+  Qed.
+
+  Lemma EU_ind' :
+    forall [φ ψ: CtlFormula] (P : ctree E C X -> Σ -> Prop),
+      (forall t s, <(t, s |= ψ)> -> P t s) -> (* base *)
+      (forall (t: ctree E C X) (s : Σ),
+          <(t, s |= φ )> ->          (* φ now*)
+          (exists t' s', ktrans (t,s) (t',s') /\ <(t',s' |= φ EU ψ)>) ->
+          (exists t' s', ktrans (t,s) (t',s') /\ P t' s') ->
+         P t s) ->
+      forall t s, <( t, s |= φ EU ψ )> -> P t s.
+  Proof.
+    intros φ ψ P Hbase Hstep.
+    refine (fix F (t : ctree E C X)(s: Σ) (H : <( t, s |= φ EU ψ)>) : P t s := _).
+    remember (entailsF φ) as p.
+    remember (entailsF ψ) as q.
+    step_entails in H.
+    dependent destruction H; subst.
+    - now apply Hbase.
+    - apply Hstep; auto.
+      destruct H0 as (t' & s' & TR & ?).
+      exists t', s'; split; auto.
+  Qed.
+
+  Lemma EF_ind' :
+    forall [φ: CtlFormula] (P : ctree E C X -> Σ -> Prop),
+      (forall t s, <(t, s |= φ)> -> P t s) -> (* base *)
+      (forall (t: ctree E C X) (s : Σ),
+          (exists t' s', ktrans (t,s) (t',s') /\ <(t',s' |= EF φ)>) ->
+          (exists t' s', ktrans (t,s) (t',s') /\ P t' s') ->
+          P t s) ->
+      forall t s, <( t, s |= EF φ )> -> P t s.
+  Proof.
+    intros φ ψ P Hbase Hstep.
+    eapply EU_ind'; eauto.
+  Qed.  
+  
   (*| [now] ignores trees and only looks at labels |*)
-  #[global] Instance proper_now: forall (p: S -> Prop) (R: relation (ctree E C X)),
-      Proper (R ==> eq ==> iff) <( now p )>.
+  #[global] Instance proper_now: forall (p: Σ -> Prop),
+      Proper (@equ E C X X eq ==> eq ==> iff) <( |- now p )>.
   Proof.
     unfold Proper, respectful, impl; cbn.      
-    intros p R x y EQ ? l <-; split; auto.
+    intros p x y EQ ? l <-; split; auto.
   Qed.
 
-  #[global] Instance proper_cand_equ (P Q: SP)
-   {PrP: Proper (@equ E C X X eq ==> eq ==> iff) P}
-   {PrQ: Proper (@equ E C X X eq ==> eq ==> iff) Q}:
-    Proper (@equ E C X X eq ==> eq ==> iff) <(P /\ Q)>.
-  Proof.
-    unfold Proper, respectful, impl, cand; cbn.
-    intros x y EQ ? l <-; split; intros (? & ?); split.
-    - now rewrite <- EQ.
-    - now rewrite <- EQ.
-    - now rewrite EQ.
-    - now rewrite EQ.
-  Qed.    
-    
-  #[global] Instance proper_cor_equ (P Q: SP)
-   {PrP: Proper (@equ E C X X eq ==> eq ==> iff) P}
-   {PrQ: Proper (@equ E C X X eq ==> eq ==> iff) Q}:
-    Proper (@equ E C X X eq ==> eq ==> iff) <(P \/ Q)>.
-  Proof.
-    unfold Proper, respectful, impl, cand; cbn.
-    intros x y EQ ? l <-; split; intros [? | ?].
-    - left; now rewrite <- EQ.
-    - right; now rewrite <- EQ.
-    - left; now rewrite EQ.
-    - right; now rewrite EQ.
-  Qed.
-  
-  #[global] Instance proper_cimpl_equ (P Q: SP)
-   {PrP: Proper (@equ E C X X eq ==> eq ==> iff) P}
-   {PrQ: Proper (@equ E C X X eq ==> eq ==> iff) Q}:
-    Proper (@equ E C X X eq ==> eq ==> iff) <(P -> Q)>.
-  Proof.
-    unfold Proper, respectful, impl, cimpl; cbn.
-    intros x y EQ ? l <-; split; intros G HP.
-    - rewrite <- EQ; apply G.
-      now rewrite EQ.
-    - rewrite EQ; apply G.
-      now rewrite <- EQ.
-  Qed.
-  
-  #[global] Instance proper_ax_equ (P: SP):
-    Proper (@equ E C X X eq ==> eq ==> iff) <( AX P )>.
-  Proof.
-    unfold Proper, respectful, impl; cbn.      
-    intros x y EQ ? l <-; split; intro NEXT;
-      unfold ax in *;
-      intros; eapply NEXT.
-    - now rewrite EQ.
-    - now rewrite <- EQ.
-  Qed.
-
-  #[global] Instance proper_ex_equ (P: SP):
-    Proper (@equ E C X X eq ==> eq ==> iff) <( EX P )>.
-  Proof.
-    unfold Proper, respectful, impl; cbn.      
-    intros x y EQ ? l <-; split; intro NEXT;
-      unfold ex in *; destruct NEXT as (l' & t' & NEXT & ?);
-      do 2 eexists; split; eauto. 
-    - now rewrite <- EQ.
-    - now rewrite EQ.
-  Qed.
-
-  #[global] Instance proper_au_equ (P Q: SP)
-   {PrP: Proper (@equ E C X X eq ==> eq ==> iff) P}
-   {PrQ: Proper (@equ E C X X eq ==> eq ==> iff) Q}:
-    Proper (@equ E C X X eq ==> eq ==> iff) <(P AU Q)>.
+  #[global] Instance proper_ret: forall (p: X -> Σ -> Prop),
+      Proper (@equ E C X X eq ==> eq ==> iff) (entailsF (CNowR p)).
   Proof.
     unfold Proper, respectful, impl; cbn.
-    intros x y EQ ? l <-; split; intro au; induction au.
-    (* -> *)
-    - rewrite EQ in H; now apply MatchA.
-    - eapply StepA.
-      + now rewrite <- EQ.
-      + intros l' t' TR.
-        eapply H0.
-        now rewrite EQ.
-    (* -> *)
-    - rewrite <- EQ in H; now apply MatchA.
-    - eapply StepA.
-      + now rewrite EQ.
-      + intros l' t' TR.
-        eapply H0.
-        now rewrite <- EQ.
+    intros; split; subst; intro; unfold entailsF in *;
+      destruct H0 as (v & ? & ?); exists v; split; auto; now rewrite <- H0.
   Qed.
-
-  #[global] Instance proper_eu_equ (P Q: SP)
-   {PrP: Proper (@equ E C X X eq ==> eq ==> iff) P}
-   {PrQ: Proper (@equ E C X X eq ==> eq ==> iff) Q}:
-    Proper (@equ E C X X eq ==> eq ==> iff) <(P EU Q)>.
-  Proof.
-    unfold Proper, respectful, impl; cbn.
-    intros x y EQ ? l <-; split; intro au; induction au.
-    (* -> *)
-    - rewrite EQ in H; now apply MatchE.
-    - eapply StepE.
-      + now rewrite <- EQ.
-      + destruct H0 as (l' & t' & TR & ?).
-        exists l', t'; split; trivial.
-        * now rewrite <- EQ.
-    (* -> *)
-    - rewrite <- EQ in H; now apply MatchE.
-    - eapply StepE.
-      + now rewrite EQ.
-      + destruct H0 as (l' & t' & TR & ?).
-        exists l', t'; split; trivial.
-        now rewrite EQ.
-  Qed.
-
-  (*| Up-to-eq enhancing function |*)
-  Variant unary_equ_clos_body (R : SP) : SP :=
-    | uEqu_clos : forall t t' s s'
-                  (Agt : t ≅ t')
-                  (HR : R t' s')
-                  (Agu : s' = s),
-        unary_equ_clos_body R t s.
-
-  Program Definition unary_equ_clos: mon SP :=
-    {| body := unary_equ_clos_body |}.
-  Next Obligation. destruct H0; econstructor; eauto. Qed.
-
-  (*| Rewrite [t ≅ u] in a CTL context t,s |= p <-> u,s |= p] |*)
-  Section gProperEqu.
-    Context {P: SP} {PrP: Proper (@equ E C X X eq ==> eq ==> iff) P}.    
-    Lemma equ_clos_ag:
-      unary_equ_clos <= agt P.
-    Proof.    
-      apply Coinduction; cbn.
-      intros R t0 s0 [t1 t2 s1 s2 EQt [Fwd Back] <-]; split.
-      - rewrite EQt; apply Fwd.
-      - intros. 
-        eapply (f_Tf (ag_ P)).
-        rewrite EQt in H.
-        apply Back in H.
-        econstructor; eauto.
-    Qed.
-
-    Lemma equ_clos_eg:
-      unary_equ_clos <= egt P.
-    Proof.    
-      apply Coinduction; cbn.
-      intros R t0 s0 [t1 t2 s1 s2 EQt [Fwd (t2' & s2' & TR & Back)] <-]; split.
-      - rewrite EQt; apply Fwd.
-      - exists t2', s2'; split.
-        + now rewrite EQt.
-        + eapply (f_Tf (eg_ P)).
-          econstructor; eauto. 
-    Qed.
-
-    #[global] Instance proper_agt_equ RR:
-      Proper (@equ E C X X eq ==> eq ==> iff) (agt P RR).
-    Proof.
-      unfold Proper, respectful, impl; cbn.
-      intros x y EQ ? l <-; split; intro G; apply (ft_t equ_clos_ag); econstructor;
-        [symmetry | apply G | reflexivity | | apply G | reflexivity]; assumption.
-    Qed.
-
-    #[global] Instance proper_agT_equ RR f:
-      Proper (@equ E C X X eq ==> eq ==> iff) (agT P f RR).
-    Proof.
-      unfold Proper, respectful, impl; cbn.
-      intros x y EQ ? l <-; split; intro G; apply (fT_T equ_clos_ag); econstructor;
-        [symmetry | apply G | reflexivity | | apply G | reflexivity]; assumption.
-    Qed.
-
-    #[global] Instance proper_ag_equ:
-      Proper (@equ E C X X eq ==> eq ==> iff) <( AG P )>.
-    Proof.
-      unfold Proper, respectful, impl; cbn.
-      intros x y EQ ? l <-; split; intro G; apply (ft_t equ_clos_ag); econstructor;
-        [symmetry | apply G | reflexivity | | apply G | reflexivity]; assumption.
-    Qed.
-    
-    #[global] Instance proper_egt_equ RR:
-      Proper (@equ E C X X eq ==> eq ==> iff) (egt P RR).
-    Proof.
-      unfold Proper, respectful, impl; cbn.
-      intros x y EQ ? l <-; split; intro G; apply (ft_t equ_clos_eg); econstructor;
-        [symmetry | apply G | reflexivity | | apply G | reflexivity]; assumption.
-    Qed.
-
-    #[global] Instance proper_egT_equ RR f:
-      Proper (@equ E C X X eq ==> eq ==> iff) (egT P f RR).
-    Proof.
-      unfold Proper, respectful, impl; cbn.
-      intros x y EQ ? l <-; split; intro G; apply (fT_T equ_clos_eg); econstructor;
-        [symmetry | apply G | reflexivity | | apply G | reflexivity]; assumption.
-    Qed.
-
-    #[global] Instance proper_eg_equ:
-      Proper (@equ E C X X eq ==> eq ==> iff) <( EG P )>.
-    Proof.
-      unfold Proper, respectful, impl; cbn.
-      intros x y EQ ? l <-; split; intro G; apply (ft_t equ_clos_eg); econstructor;
-        [symmetry | apply G | reflexivity | | apply G | reflexivity]; assumption.
-    Qed.
-
-    (* Allow rewriting under entailment *)
-    #[global] Instance proper_entails_equ:
-      Proper (@equ E C X X eq ==> @eq S ==> iff) (entails P). 
-    Proof.
-      unfold Proper, respectful, iff;
-        intros x y EQx a ? <-; split; intro G; unfold entails in *; [now rewrite <- EQx | now rewrite EQx].
-    Qed.
-  End gProperEqu.
-                
+  
   (*| Up-to-sbisim enhancing function |*)
-  Variant unary_sbisim_clos_body (R : SP) : SP :=
+  Variant unary_sbisim_clos_body (R: rel (ctree E C X) Σ) : rel (ctree E C X) Σ :=
     | uSbisim_clos : forall t t' s s'
                   (Agt : t ~ t')
                   (HR : R t' s')
                   (Agu : s' = s),
         unary_sbisim_clos_body R t s.
 
-  Program Definition unary_sbisim_clos: mon SP :=
+  Program Definition unary_sbisim_clos: mon (rel (ctree E C X) Σ) :=
     {| body := unary_sbisim_clos_body |}.
   Next Obligation. destruct H0; econstructor; eauto. Qed.
 
-  (*| Rewrite [t ~ u] in a CTL context t,s |= p <-> u,s |= p] |*)
+  (** Rewrite [t ~ u] in a CTL context t,s |= p <-> u,s |= p] *)
   Section gProperSbisim.
-    Context {P: SP} {PrP: Proper (@sbisim E E C C X X _ _ eq ==> eq ==> iff) P}.
+    Context {P Q: rel (ctree E C X) Σ}
+            {PrP: Proper (@sbisim E E C C X X _ _ eq ==> eq ==> iff) P}
+            {PrQ: Proper (@sbisim E E C C X X _ _ eq ==> eq ==> iff) Q}.
     
-    Lemma sbisim_clos_ag:
-      unary_sbisim_clos <= agt P.
+    Lemma sbisim_clos_car:
+      unary_sbisim_clos <= cart P Q.
     Proof.    
       apply Coinduction; cbn.
-      intros R t0 s0 [t1 t2 s1 s2 EQt [Fwd Back] <-]; split.
-      - rewrite EQt; apply Fwd.
-      - intros. 
-        eapply (f_Tf (ag_ P)).
-        rewrite <- EQt in Fwd.
-        destruct (ktrans_sbisim_l H EQt) as (? & ? & ?); eauto.
+      intros R t0 s0 [t1 t2 s1 s2 EQt HH]; inv HH.
+      - now apply RMatchA; rewrite EQt. 
+      - apply RStepA; [now rewrite EQt|].
+        intros t' s' Fwd.
+        eapply (f_Tf (car P Q)).
+        destruct (ktrans_sbisim_l Fwd EQt) as (? & ? & ?); eauto.        
         econstructor.
-        + apply H1.
-        + apply Back.
-          apply H0.
+        + apply H2.
+        + apply H0; eassumption.
         + reflexivity.
     Qed.
 
-    Lemma sbisim_clos_eg:
-      unary_sbisim_clos <= egt P.
+    Lemma sbisim_clos_cer:
+      unary_sbisim_clos <= cert P Q.
     Proof.    
       apply Coinduction; cbn.
-      intros R t0 s0 [t1 t2 s1 s2 EQt [Fwd Back] <-]; split.
-      - rewrite EQt; apply Fwd.
-      - destruct Back as (t2' & s2' & TR2 & ?).
+      intros R t0 s0 [t1 t2 s1 s2 EQt HH]; inv HH.
+      - now apply RMatchE; rewrite EQt. 
+      - destruct H0 as (t2' & s2' & TR2 & ?).
         symmetry in EQt.
-        destruct (ktrans_sbisim_l TR2 EQt) as (? & ? & ?); eauto.
-        exists x, s2'; intuition.
-        eapply (f_Tf (eg_ P)).
-        symmetry in H1.
-        econstructor; eauto.
+        destruct (ktrans_sbisim_l TR2 EQt) as (t1' & TR1' & EQt1'); eauto.
+        apply RStepE.
+        + now rewrite <- EQt.
+        + exists t1', s2'; intuition.
+          eapply (f_Tf (cer P Q)).
+          symmetry in EQt1'.
+          econstructor; eauto.
     Qed.
-    
-    #[global] Instance proper_egt_sbisim RR:
-      Proper (sbisim eq ==> eq ==> iff) (egt P RR).
+
+    #[global] Instance proper_ewt_sbisim RR:
+      Proper (sbisim eq ==> eq ==> iff) (cert P Q RR).
     Proof.
       unfold Proper, respectful, impl; cbn.
-      intros x y EQ ? l <-; split; intro G; apply (ft_t sbisim_clos_eg); econstructor;
+      intros x y EQ ? l <-; split; intro G; apply (ft_t sbisim_clos_cer); econstructor;
         [symmetry | apply G | reflexivity | | apply G | reflexivity]; assumption.
     Qed.
 
-    #[global] Instance proper_egT_sbisim RR f:
-      Proper (sbisim eq ==> eq ==> iff) (egT P f RR).
+    #[global] Instance proper_ewT_sbisim RR f:
+      Proper (sbisim eq ==> eq ==> iff) (cerT P Q f RR).
     Proof.
       unfold Proper, respectful, impl; cbn.
-      intros x y EQ ? l <-; split; intro G; apply (fT_T sbisim_clos_eg); econstructor;
-        [symmetry | apply G | reflexivity | | apply G | reflexivity]; assumption.
-    Qed.
-
-    #[global] Instance proper_eg_sbisim:
-      Proper (sbisim eq ==> eq ==> iff) <( EG P )>.
-    Proof.
-      unfold Proper, respectful, impl; cbn.
-      intros x y EQ ? l <-; split; intro G; apply (ft_t sbisim_clos_eg); econstructor;
+      intros x y EQ ? l <-; split; intro G; apply (fT_T sbisim_clos_cer); econstructor;
         [symmetry | apply G | reflexivity | | apply G | reflexivity]; assumption.
     Qed.
         
-    #[global] Instance proper_agt_sbisim RR:
-      Proper (sbisim eq ==> eq ==> iff) (agt P RR).
+    #[global] Instance proper_awt_sbisim RR:
+      Proper (sbisim eq ==> eq ==> iff) (cart P Q RR).
     Proof.
       unfold Proper, respectful, impl; cbn.
-      intros x y EQ ? l <-; split; intro G; apply (ft_t sbisim_clos_ag); econstructor;
+      intros x y EQ ? l <-; split; intro G; apply (ft_t sbisim_clos_car); econstructor;
         [symmetry | apply G | reflexivity | | apply G | reflexivity]; assumption.
     Qed.
 
-    #[global] Instance proper_agT_sbisim RR f:
-      Proper (sbisim eq ==> eq ==> iff) (agT P f RR).
+    #[global] Instance proper_awT_sbisim RR f:
+      Proper (sbisim eq ==> eq ==> iff) (carT P Q f RR).
     Proof.
       unfold Proper, respectful, impl; cbn.
-      intros x y EQ ? l <-; split; intro G; apply (fT_T sbisim_clos_ag); econstructor;
+      intros x y EQ ? l <-; split; intro G; apply (fT_T sbisim_clos_car); econstructor;
         [symmetry | apply G | reflexivity | | apply G | reflexivity]; assumption.
     Qed.
 
-    #[global] Instance proper_ag_sbisim:
-      Proper (sbisim eq ==> eq ==> iff) <( AG P )>.
+    #[global] Instance proper_cer_sbisim:
+      Proper (sbisim eq ==> eq ==> iff) (gfp (cer P Q)).
     Proof.
       unfold Proper, respectful, impl; cbn.
-      intros x y EQ ? l <-; split; intro G; apply (ft_t sbisim_clos_ag); econstructor;
+      intros x y EQ ? l <-; split; intro G; apply (ft_t sbisim_clos_cer); econstructor;
         [symmetry | apply G | reflexivity | | apply G | reflexivity]; assumption.
     Qed.
 
-    (* Allow rewriting under entailment *)
-    #[global] Instance proper_entails_sbisim:
-      Proper (sbisim eq ==> eq ==> iff) (entails P). 
+    #[global] Instance proper_car_sbisim:
+      Proper (sbisim eq ==> eq ==> iff) (gfp (car P Q)).
     Proof.
-      unfold Proper, respectful, iff;
-        intros x y EQx a ? <-; split; intro G; unfold entails in *; [now rewrite <- EQx | now rewrite EQx].
+      unfold Proper, respectful, impl; cbn.
+      intros x y EQ ? l <-; split; intro G; apply (ft_t sbisim_clos_car); econstructor;
+        [symmetry | apply G | reflexivity | | apply G | reflexivity]; assumption.
     Qed.
+
   End gProperSbisim.
 
-  (*| Up-to-bind ag |*)
-  Section gProperBind.
-    Context {Y: Type}.
+    (*| Up-to-eq enhancing function |*)
+  Variant unary_equ_clos_body (R : rel (ctree E C X) Σ) : rel (ctree E C X) Σ :=
+    | uEqu_clos : forall t t' s s'
+                  (Agt : t ≅ t')
+                  (HR : R t' s')
+                  (Agu : s' = s),
+        unary_equ_clos_body R t s.
 
-    Print SP.
-    Print ag.
-    (*| Up-to-bind enchancing function (unary context) |*)
-    Definition bind_clos
-               (R: rel (ctree E C X) S)
-               (Rk: (X -> ctree E C Y) -> Prop):
-      rel (ctree E C Y) S :=
+  Program Definition unary_equ_clos: mon (rel (ctree E C X) Σ) :=
+    {| body := unary_equ_clos_body |}.
+  Next Obligation. destruct H0; econstructor; eauto. Qed.
+
+  (*| Rewrite [t ≅ u] in a CTL context t,s |= p <-> u,s |= p] |*)
+  Section gProperEqu.
+    Context {P Q: rel (ctree E C X) Σ}
+            {PrP: Proper (@equ E C X X eq ==> eq ==> iff) P}
+            {PrQ: Proper (@equ E C X X eq ==> eq ==> iff) Q}.    
+    Lemma equ_clos_car:
+      unary_equ_clos <= cart P Q.
+    Proof.    
+      apply Coinduction; cbn.
+      intros R t0 s0 [t1 t2 s1 s2 EQt HH]; inv HH.
+      - apply RMatchA; now rewrite EQt. 
+      - apply RStepA; intros.
+        + now rewrite EQt.
+        + eapply (f_Tf (car P Q)).
+          econstructor; eauto.
+          apply H0.
+          now rewrite <- EQt.
+    Qed.
+
+    Lemma equ_clos_cer:
+      unary_equ_clos <= cert P Q.
+    Proof.    
+      apply Coinduction; cbn.
+      intros R t0 s0 [t1 t2 s1 s2 EQt HH]; inv HH. 
+      - apply RMatchE; now rewrite EQt. 
+      - destruct H0 as (u & x & TR2 & ?).
+        apply RStepE.
+        + now rewrite EQt.
+        + exists u, x; intuition.
+          now rewrite EQt.
+          eapply (f_Tf (cer P Q)).
+          econstructor; eauto. 
+    Qed.
+
+    #[global] Instance proper_cart_equ RR:
+      Proper (@equ E C X X eq ==> eq ==> iff) (cart P Q RR).
+    Proof.
+      unfold Proper, respectful, impl; cbn.
+      intros x y EQ ? l <-; split; intro G; apply (ft_t equ_clos_car); econstructor;
+        [symmetry | apply G | reflexivity | | apply G | reflexivity]; assumption.
+    Qed.
+
+    #[global] Instance proper_carT_equ RR f:
+      Proper (@equ E C X X eq ==> eq ==> iff) (carT P Q f RR).
+    Proof.
+      unfold Proper, respectful, impl; cbn.
+      intros x y EQ ? l <-; split; intro G; apply (fT_T equ_clos_car); econstructor;
+        [symmetry | apply G | reflexivity | | apply G | reflexivity]; assumption.
+    Qed.
+    
+    #[global] Instance proper_cert_equ RR:
+      Proper (@equ E C X X eq ==> eq ==> iff) (cert P Q RR).
+    Proof.
+      unfold Proper, respectful, impl; cbn.
+      intros x y EQ ? l <-; split; intro G; apply (ft_t equ_clos_cer); econstructor;
+        [symmetry | apply G | reflexivity | | apply G | reflexivity]; assumption.
+    Qed.
+
+    #[global] Instance proper_cerT_equ RR f:
+      Proper (@equ E C X X eq ==> eq ==> iff) (cerT P Q f RR).
+    Proof.
+      unfold Proper, respectful, impl; cbn.
+      intros x y EQ ? l <-; split; intro G; apply (fT_T equ_clos_cer); econstructor;
+        [symmetry | apply G | reflexivity | | apply G | reflexivity]; assumption.
+    Qed.
+
+    #[global] Instance proper_cer_equ:
+      Proper (@equ E C X X eq ==> eq ==> iff) (gfp (cer P Q)).
+    Proof.
+      unfold Proper, respectful, impl; cbn.
+      intros x y EQ ? l <-; split; intro G; apply (ft_t equ_clos_cer); econstructor;
+        [symmetry | apply G | reflexivity | | apply G | reflexivity]; assumption.
+    Qed.
+
+    #[global] Instance proper_car_equ:
+      Proper (@equ E C X X eq ==> eq ==> iff) (gfp (car P Q)).
+    Proof.
+      unfold Proper, respectful, impl; cbn.
+      intros x y EQ ? l <-; split; intro G; apply (ft_t equ_clos_car); econstructor;
+        [symmetry | apply G | reflexivity | | apply G | reflexivity]; assumption.
+    Qed.
+
+    #[global] Instance proper_cau_equ:
+      Proper (@equ E C X X eq ==> eq ==> iff) (cau P Q).
+    Proof.
+      unfold Proper, respectful, impl; cbn.
+      intros x y EQ ? l <-; split; intro au; induction au.
+      (* -> *)
+      - rewrite EQ in H; now apply MatchA.
+      - eapply StepA.
+        + now rewrite <- EQ.
+        + intros l' t' TR.
+          eapply H0.
+          now rewrite EQ.
+      (* -> *)
+      - rewrite <- EQ in H; now apply MatchA.
+      - eapply StepA.
+        + now rewrite EQ.
+        + intros l' t' TR.
+          eapply H0.
+          now rewrite <- EQ.
+    Qed.
+
+    #[global] Instance proper_ceu_equ:
+      Proper (@equ E C X X eq ==> eq ==> iff) (ceu P Q).
+    Proof.
+      unfold Proper, respectful, impl; cbn.
+      intros x y EQ ? l <-; split; intro au; induction au.
+      (* -> *)
+      - rewrite EQ in H; now apply MatchE.
+      - eapply StepE.
+        + now rewrite <- EQ.
+        + destruct H0 as (l' & t' & TR & ?).
+          exists l', t'; split; trivial.
+          * now rewrite <- EQ.
+      (* -> *)
+      - rewrite <- EQ in H; now apply MatchE.
+      - eapply StepE.
+        + now rewrite EQ.
+        + destruct H0 as (l' & t' & TR & ?).
+          exists l', t'; split; trivial.
+          now rewrite EQ.
+    Qed.
+    
+  End gProperEqu.
+  
+  (*| Combined Properness lemma without the properness requirements, by induction on formulas |*)
+  #[global] Instance proper_equiv_equ:
+    Proper (equiv ==> equ eq ==> eq ==> iff) (@entailsF E C X Σ h HasStuck).
+  Proof.
+    do 4 red; intro x; induction x; intros y Hy t u EQt s s' <-; rewrite <- (Hy u s); clear Hy; step_entails; auto;
+    try (specialize (IHx1 x1 (setoid_refl _ x1));        
+         replace (forall x y : ctree E C X, x ≅ y -> forall x0 y0 : Σ, x0 = y0 -> <( x, x0 |= x1 )> <-> <( y, y0 |= x1 )>) with
+           (Proper (equ eq ==> eq ==> iff) (@entailsF E C X Σ h HasStuck x1)) in IHx1 by reflexivity);
+    try (specialize (IHx2 x2 (setoid_refl _ x2));        
+         replace (forall x y : ctree E C X, x ≅ y -> forall x0 y0 : Σ, x0 = y0 -> <( x, x0 |= x2 )> <-> <( y, y0 |= x2 )>) with
+           (Proper (equ eq ==> eq ==> iff) (@entailsF E C X Σ h HasStuck x2)) in IHx2 by reflexivity).
+    - (* ret *)
+      split; intros (? & ? & ?); eauto. 
+      + exists x; rewrite EQt in H; intuition.
+      + exists x; rewrite EQt; intuition.
+    - (* /\ *)
+      split; intros (? & ?); split.
+      + now rewrite <- EQt. 
+      + now rewrite <- EQt. 
+      + now rewrite EQt. 
+      + now rewrite EQt. 
+    - (* \/ *)
+      split; intros [? | ?].
+      + now left; rewrite <- EQt. 
+      + now right; rewrite <- EQt. 
+      + now left; rewrite EQt. 
+      + now right; rewrite EQt. 
+    - (* -> *)
+      split; intros.
+      + rewrite <- EQt; rewrite <- EQt in H0; auto.
+      + rewrite EQt; rewrite EQt in H0; auto.
+    - (* ax *)
+      split; intros.
+      + now rewrite <- EQt in H0; apply H in H0.
+      + now rewrite EQt in H0; apply H in H0.
+    - (* ex *)
+      split; intros (t' & x' & ? & ?); do 2 eexists; split; eauto.
+      + now rewrite <- EQt.
+      + now rewrite EQt.
+    - (* au *)
+      now rewrite EQt.
+    - (* eu *)
+      now rewrite EQt.
+    - (* aw *)
+      now rewrite EQt.
+    - (* ew *)
+      now rewrite EQt.
+  Qed.
+
+  (*| Up-to-bind ag |*)
+  Definition bind_clos {Y}
+             (R: rel (ctree E C X) Σ)
+             (Rk: (X -> ctree E C Y) -> Prop):
+      rel (ctree E C Y) Σ :=
       sup_all (fun t => sup (R t)
                          (fun s' => sup Rk
                                      (fun k => pairH (CTree.bind t k) s'))).
   
     (*| Specialization of [bind_ctx] to a function acting with [equ] on the bound value,
         and with the argument (pointwise) on the continuation. |*)
-    Program Definition bind_clos_ag p: mon (rel (ctree E C Y) S) :=
-      {| body := fun R => bind_clos (ag p) (fun k => forall x s, R (k x) s) |}.
+    Program Definition bind_clos_ag Y p q: mon (rel (ctree E C Y) Σ) :=
+      {| body := fun R => bind_clos (gfp (car p q)) (fun k => forall x s, R (k x) s) |}.
     Next Obligation.
       (* TODO *)
       (* unfold bind_clos.
       apply leq_bind_ctx. intros ?? H' ?? H''.
       apply in_bind_ctx. apply H'. intros t t' HS. apply H0, H'', HS. *)
     Admitted.
-  End gProperBind.
 End Equivalences.
 
 (*| Ltac Tactics |*)
-#[local] Ltac __fold_g :=
-  repeat
-    match goal with
-    | h: context[@ag_ ?E ?C ?S ?X ?h ?HS ?R ] |- _ => fold (@ag E C S X h HS R) in h
-    | |- context[@ag_ ?E ?C ?S ?X ?h ?HS ?R ]      => fold (@ag E C S X h HS R)
-    | h: context[@eg_ ?E ?C ?S ?X ?h ?HS ?R ] |- _ => fold (@eg E C S X h HS R) in h
-    | |- context[@eg_ ?E ?C ?S ?X ?h ?HS ?R ]      => fold (@eg E C S X h HS R)
-    end.
-
-#[local] Ltac __fold_entails :=  
-  lazymatch goal with
-  | |- context[entails ?ϕ ?t ?s] => fail "Already in [t, s |= p] form"
-  | |- context[?ϕ ?t ?s] =>
-      match type of ϕ with
-      |_ -> _ -> Prop =>
-         match type of t with
-         | ctree ?E ?C ?X =>
-             replace (ϕ t s) with (entails ϕ t s) by reflexivity
-         end
-      end                
+#[local] Ltac __step_formula E C X S h HasStuck φ :=
+  lazymatch φ with
+  | context[CAU ?p ?q] => lazymatch eval cbv in p with
+                         | CNowS (fun _ => True) => rewrite (@ctl_af_ax E C X S HasStuck h)
+                         | _ => rewrite (@ctl_au_ax E C X S HasStuck h)
+                         end
+  | context[CEU ?p ?q] => lazymatch eval cbv in p with
+                         | CNowS (fun _ => True) => rewrite (@ctl_ef_ex E C X S HasStuck h)
+                         | _ => rewrite (@ctl_eu_ex E C X S HasStuck h)
+                         end
+  | context[CAR ?p ?q] => lazymatch eval cbv in p with
+                         | CNowS (fun _ => False) => rewrite (@ctl_ag_ax E C X S HasStuck h)
+                         | _ => rewrite (@ctl_ar_ax E C X S HasStuck h)
+                         end
+  | context[CER ?p ?q] => lazymatch eval cbv in p with
+                         | CNowS (fun _ => False) => rewrite (@ctl_eg_ex E C X S HasStuck h)
+                         | _ => rewrite (@ctl_er_ex E C X S HasStuck h)
+                         end
+  | CAX ?p => step_entails;
+             let t_ := fresh "t" in
+             let s_ := fresh "s" in
+             let TR_ := fresh "TR" in
+             intros t_ s_ TR_
+  | CEX ?p => step_entails
+  | ?ptrivial => lazymatch eval compute in ptrivial with
+                | CNowS ?f => step_entails
+                | _ => fail "Cannot step formula " φ
+                end
   end.
 
-#[local] Ltac __fold_entails_in H :=
-  lazymatch type of H with
-  | context[entails ?ϕ ?t ?s] => fail "Already in [t, s |= p] form"
-  | context[?ϕ ?t ?s] =>
-       match type of ϕ with
-       |ctree ?E ?C ?X -> ?S -> Prop =>
-         match type of t with
-         | ctree ?E ?C ?X =>
-             match type of s with
-             | ?S => replace (ϕ t s) with (entails ϕ t s) in H by reflexivity
-             end
-         end
-      end                
-  end.
-
-#[local] Tactic Notation "__step_x" :=
-  lazymatch goal with
-  | |- entails (@ax ?E ?C ?X ?S ?h ?HasStuck ?p) ?t ?s =>
-      unfold entails, ax;
-      repeat (
-          let t_ := fresh "t" in
-          let s_ := fresh "s" in
-          let TR_ := fresh "TR" in
-          intros t_ s_ TR_)
-  | |- entails (@ex ?E ?C ?X ?S ?h ?HasStuck ?p) ?t ?s =>
-      unfold entails, ex; do 2 eexists
-  end; __fold_entails.
-
-#[local] Ltac __step_in_x H :=
-  lazymatch type of H with
-  | entails (@ax ?E ?C ?X ?S ?h ?HasStuck ?p) ?t ?s =>
-      unfold entails, ax in H;
-      lazymatch goal with
-      | H: forall t' : ctree ?E ?C ?X, forall s': ?S, ktrans ?L (t', s') -> ?ϕ t' s' |- _ => 
-          lazymatch type of ϕ with
-          |_ -> _ -> Prop =>
-             replace (forall (t' : ctree E C X) (s': S) , ktrans L (t', s') -> ϕ t' s') with
-             (forall (t' : ctree E C X) (s': S) , ktrans L (t', s') -> entails ϕ t' s') in H by reflexivity
-          end
-      end
-  | entails (@ex ?E ?C ?X ?S ?h ?HasStuck ?p) ?t ?s =>
+#[local] Ltac __step_formula_in H E C X S h HasStuck φ :=
+  lazymatch φ with
+  | context[CAU ?p ?q] => lazymatch eval cbv in p with
+                         | CNowS (fun _ => True) => rewrite (@ctl_af_ax E C X S HasStuck h) in H
+                         | _ => rewrite (@ctl_au_ax E C X S HasStuck h) in H
+                         end
+  | context[CEU ?p ?q] => lazymatch eval cbv in p with
+                         | CNowS (fun _ => True) => rewrite (@ctl_ef_ex E C X S HasStuck h) in H
+                         | _ => rewrite (@ctl_eu_ex E C X S HasStuck h) in H
+                         end
+  | context[CAR ?p ?q] => lazymatch eval cbv in p with
+                         | CNowS (fun _ => False) => rewrite (@ctl_ag_ax E C X S HasStuck h) in H
+                         | _ => rewrite (@ctl_ar_ax E C X S HasStuck h) in H
+                         end
+  | context[CER ?p ?q] => lazymatch eval cbv in p with
+                         | CNowS (fun _ => False) => rewrite (@ctl_eg_ex E C X S HasStuck h) in H
+                         | _ => rewrite (@ctl_er_ex E C X S HasStuck h) in H
+                         end
+  | CAX ?p => step_entails in H
+  | CEX ?p =>
       let t_ := fresh "t" in
       let s_ := fresh "s" in
       let TR_ := fresh "TR" in
       let NOW_ := fresh "Hnow" in
-      unfold entails, ex in H; destruct H as (t_ & s_ & TR_ & NOW_);
-      replace (p t_ s_) with (entails p t_ s_) in NOW_ by reflexivity
+      destruct H as (t_ & s_ & TR_ & NOW_);
+      fold (@entailsF E C X S h HasStuck) in NOW_
+  | ?ptrivial => lazymatch eval compute in ptrivial with
+                | CNowS ?f => step_entails in H
+                | _ => fail "Cannot step formula " φ " in " H
+                end
   end.
 
-#[local] Tactic Notation "__step_u" :=
-  lazymatch goal with
-  | |- entails (@au ?E ?C ?X ?S ?h ?HasStuck ?p ?q) ?t ?s =>
-      unfold entails; apply ctl_au_ax
-  | |- entails (@eu ?E ?C ?X ?S ?h ?HasStuck ?p ?q) ?t ?s =>
-      unfold entails; apply ctl_eu_ex
-  end; __fold_entails.
-
-#[local] Ltac __step_in_u H :=
-  lazymatch type of H with
-  | entails (@au ?E ?C ?X ?S ?h ?HasStuck ?p ?q) ?t ?s =>
-      let NOW_ := fresh "Hnow" in
-      unfold entails; apply ctl_au_ax in H; destruct H;
-      [|destruct H as (NOW_ & ?); __fold_entails_in NOW_]
-  | entails (@eu ?E ?C ?X ?S ?h ?HasStuck ?p ?q) ?t ?s =>
-      unfold entails, ex; apply ctl_eu_ex in H
-  end; __fold_entails_in H.
-
-#[local] Tactic Notation "__step_g" :=
-  lazymatch goal with
-  | |- entails (@ag ?E ?C ?S ?X ?h ?HasStuck ?p) ?t ?q =>
-      unfold entails, ag;
-      step;
-      fold (@ag E C S X h HasStuck p t q)
-  | |- entails (@eg ?E ?C ?S ?X ?h ?HasStuck ?p) ?t ?q =>
-      unfold entails,eg;
-      step;
-      fold (@eg E C S X h HasStuck p t q)
-  end;  __fold_entails.
-
-#[local] Ltac __step_in_g H :=
-  lazymatch type of H with
-  | entails (@ag ?E ?C ?S ?X ?h ?HasStuck ?p) ?t ?s =>
-      unfold entails, ag in H;
-      step in H;
-      fold (@ag E C S X h HasStuck) in H
-  | entails (@eg ?E ?C ?S ?X ?h ?HasStuck ?p) ?t ?s =>
-      unfold entails, eg in H;
-      step in H;
-      fold (@eg E C S X h HasStuck) in H
-  end; __fold_entails_in H.
-
 #[local] Ltac __coinduction_g R H :=
-  unfold entails, ag, eg; coinduction R H; __fold_g; __fold_entails.
+  step_entails; coinduction R H.
 
 (** Re-export [Eq.v] tactics *)
 #[global] Tactic Notation "step" :=
-  __step_x || __step_u || __step_g || step.
+  lazymatch goal with
+  | |- context[@entailsF ?E ?C ?X ?S ?h ?HasStuck ?p ?t ?s] =>
+      __step_formula E C X S h HasStuck p
+  end || step.
 
 #[global] Tactic Notation "coinduction" simple_intropattern(R) simple_intropattern(H) :=
   __coinduction_g R H || coinduction R H.
 
 #[global] Tactic Notation "step" "in" ident(H) :=
-  __step_in_x H || __step_in_u H || __step_in_g H || step_in H.
-
-Tactic Notation "right" := right; try progress __fold_entails.
-Tactic Notation "left" := left; try progress __fold_entails.
-Tactic Notation "split" := split; try progress __fold_entails.
+  lazymatch type of H with
+  | context[@entailsF ?E ?C ?X ?S ?h ?HasStuck ?p ?s ?t] =>
+      __step_formula_in H E C X S h HasStuck p
+  end || step_in H.
 
 Section UsefulLemmas.
   Import CtlNotations CTreeNotations.
   Local Open Scope ctl_scope.
-
-  Context {E C: Type -> Type} {X S: Type} {HasStuck: B0 -< C} {h: Handler E S}.
-  Notation SP := (ctree E C X -> S -> Prop).
   
-  Lemma ctl_ret_au_inv: forall x s (p q: S -> Prop),
-      <( {Ret x: ctree E C X}, s |= (now p) AU (now q) )> -> p s \/ q s.
+  Lemma ctl_ret_au_inv {E C X Σ} {HasStuck: B0 -< C} {h: Handler E Σ}: forall x s (p q: Σ -> Prop),
+      <( {Ret x: ctree E C X}, s |= (now p) AU (now q)  )> -> p s \/ q s.
   Proof.
-    intros.
-    step in H; [now right | now left].
+    intros; inv H; [now right | now left].
   Qed.
 
-  Lemma ctl_bind_au_inv: forall p q (t: ctree E C X) (s: S) (k: X -> ctree E C X),
-      <( {x <- t ;; k x}, s |= (now p) AU (now q) )> ->
-      <( t,s |= (now p) AU (ret {fun x s => <( {k x}, s |= (now p) AU (now q) )>}) )> \/
-        <( t,s |= (now p) AU (now q) )>.
+  Lemma ctl_bind_au_inv{E C X Σ Y} {HasStuck: B0 -< C} {h: Handler E Σ}: forall (φ ψ: Σ -> Prop) (t: ctree E C Y) (s: Σ) (k: Y -> ctree E C X),
+      <( {x <- t ;; k x}, s |= (now φ) AU (now ψ) )> <->
+      <( t,s |= (now φ) AU (ret {fun x s => <( {k x}, s |= (now φ) AU (now ψ) )>}) )> \/ 
+        <( t,s |= (now φ) AU (now ψ) )>.
   Proof.
     intros.
-    unfold entails in H.
-    inv H.
-    - admit.
-    - admit.
+    remember (CNowS φ).
+    remember (CNowS ψ).
   Admitted.
+
+  Lemma ctl_bind_ag_goal{E C X Σ Y} {HasStuck: B0 -< C} {h: Handler E Σ}: forall φ (t: ctree E C Y) (s: Σ) (k: Y -> ctree E C X),
+      <( {x <- t ;; k x}, s |= AG (now φ) )> <->
+      <( t,s |= (ret {fun x s => <( {k x}, s |= AG (now φ) )>}) AR (now φ) )>.
+  Proof.
+    intros.
+    remember (CNowS φ).
+  Admitted.
+
 End UsefulLemmas.
 
 (* Examples *)
 From CTree Require Import
      FoldStateT.
 
+
 Module Experiments.
 
   Import CTree CTreeNotations CtlNotations.
   Local Open Scope ctl_scope.
-
-  (* Dummy program *)
-  Definition dummy_23 : ctree (stateE nat) B0 unit :=
-    put 2 ;;
-    put 3.
-
-  (* Why ctl_of_State did not register? Nvm, it's too general... *)
-  Print Coercions.
-  Section COERC.
-    Context {C: Type -> Type} {X: Type}.
-    Notation SP := (ctree (stateE nat) C X -> nat -> Prop).
-    Definition ctl_of_State (s: nat): SP := nowS (fun x => x = s).
-    Arguments ctl_of_State /.
-    Coercion ctl_of_State : nat >-> Funclass.
-  End COERC.
+  Context {E C: Type -> Type} {S: Type} {HasStuck: B0 -< C}.
+  Definition stuck: ctree E C unit := stuckD.
+    
+  Definition ctl_of_State {X}(s: nat): @CtlFormula X nat := CNowS (fun x => x = s).
+  Arguments ctl_of_State /.
+  Coercion ctl_of_State : nat >-> CtlFormula.
 
   Lemma writes_23: forall s,
-      <( dummy_23, s |= AX 2 /\ (AX (AX 3)) )>.
+      <( {put 2 ;; put 3 : ctree (stateE nat) B0 unit}, s |= AX 2 /\ (AX (AX 3)) )>.
   Proof.
-    unfold dummy_23.
-    split.
+    split; intros; fold_entails.
     - step.
-      apply ktrans_trigger_inv in TR as ([] & ? & ->).
+      apply ktrans_trigger_inv in H as ([] & ? & ->).
       cbn; auto.
     - step.  
-      apply ktrans_trigger_inv in TR as ([] & ? & ->).
+      apply ktrans_trigger_inv in H as ([] & ? & ->).
       rewrite H in *; clear H.
-      apply ktrans_vis_inv in TR0 as ([] & -> & ->).
+      apply ktrans_vis_inv in H0 as ([] & ? & ->).
       cbn; auto.
   Qed.      
 
-  Context {E C: Type -> Type} {X S: Type} {HasStuck: B0 -< C} {h: Handler E S}.
-  Definition stuck: ctree E C X := stuckD.
-    
-  Ltac shallow_inv_trans H1 := unfold trans,transR in H1; cbn in H1; dependent destruction H1.
-  
-  Lemma is_stuck_ax: forall (s: S),
+  Lemma is_stuck_ax: forall (s: S) {h: Handler E S},
       <( stuck, s |= (AX False) )>.
   Proof.
-    unfold cimpl, ax, entails. intros.
-    inv H.
-    1,2: shallow_inv_trans H1; contradiction.
-    all: shallow_inv_trans H3; contradiction. 
+    intros.
+    step.
+    now apply ktrans_stuck_inv in TR.
   Qed.
 
   (* Terminating [ret x] programs *)
-  Definition put2: ctree (stateE nat) C unit := put 2.
-  
   Lemma maybebad: forall n,
-      <( put2, n |= AF 3 )>.
+      ~ <( {put 2: ctree (stateE nat) C unit}, n |= AX 3 )>.
   Proof.
-    unfold entails.
-    right; eauto.
-    intros.
-    inv H.
-    - shallow_inv_trans H1.
-    - apply trans_vis_inv in H1 as ([] & ? & ?).
-      dependent destruction H0.
-      cbn.
-      rewrite H.
-      (* Ret tt *)
-      right; eauto.
-      intros; clear H t'.
-      apply ktrans_ret in H0 as (-> & <-).
-      apply StepA; auto.
-      intros.
-      (* Same [Ret tt] as before, and it will keep being [Ret tt] *)
-   Abort.
+    intros * CONTRA.
+    step in CONTRA.
+    assert (TR: @ktrans _ C _ _ _ _ (put 2, n) (Ret tt, 2)).
+    eapply ktrans_vis_goal; intuition.
+    apply CONTRA in TR.
+    discriminate TR.
+  Qed.
 
   Lemma maybegood: forall n,
-      <( put2, n |= AF 2 )>.
+      <( {put 2: ctree (stateE nat) C unit}, n |= AF 2 )>.
   Proof.
-    unfold entails.
-    right; eauto.
     intros.
-    inv H.
-    - shallow_inv_trans H1.
-    - apply trans_vis_inv in H1 as ([] & ? & ?).
-      dependent destruction H0.      
-      rewrite H.
-      left; cbn.
-      trivial.
-    - inv H3.
+    step; right; intros.
+    apply MatchA; cbn.
+    apply ktrans_vis_inv in H as ([] & ? & ->).
+    reflexivity.
   Qed.
+
   
   Lemma maybegood': 
-    <( put2, 2 |= AG 2 )>.
+    <( {put 2: ctree (stateE nat) C unit}, 2 |= AG 2 )>.
   Proof.
-    unfold entails.
-    apply ctl_ag_ax; split.
-    - trivial.
-    - unfold put2; step.
-      apply ktrans_vis_inv in TR as ([] & -> & ->).
-      cbn.
-      coinduction R CIH.
-      econstructor; trivial.
-      intros.
-      apply ktrans_ret in H as (-> & <-).
-      apply CIH.
-      auto.
+    step.
+    split; auto; cbn.
+    intros.
+    apply ktrans_vis_inv in H as ([] & ? & ->).
+    (* Why this instance cannot be found ? *)
+    pose proof (@proper_car_equ (stateE nat) C unit nat _ _ <( |- now {fun _ => False} )> <( |- now {fun s => s = 2} )> (proper_now _) (proper_now _)).
+    rewrite H.
+    coinduction R CIH.
+    
+    apply RStepA; auto; cbn in *.
+    intros.
+    apply ktrans_ret in H1 as (? & <-).
+    pose proof (@proper_cart_equ (stateE nat) C unit nat _ _ <( |- now {fun _ => False} )> <( |- now {fun s => s = 2} )> (proper_now _) (proper_now _) R).
+    rewrite H1.
+    apply CIH.
+    exact t'.
   Qed.
 
   Lemma maybegood'': 
-    ~ <( put2, 2 |= AG 3 )>.
+    ~ <( {put 2: ctree (stateE nat) C unit}, 2 |= AG 3 )>.
   Proof.
-    unfold entails.
     unfold not.
     intro CONTRA.
     step in CONTRA; inv CONTRA.
     inv H.
   Qed.
-
-  Lemma ag_forever': forall (t: ctree E C X) (s: S) p {HasTau: B1 -< C},
-      <( t, s |= now p )> -> <( {forever t: ctree E C X},s |= AG now p )>.
-  Proof.
-    unfold entails; intros; coinduction R CIH.
-    - econstructor.
-      rewrite unfold_forever.
-
-  Admitted.
 
 End Experiments.
 
